fstar/new/MLS.Test.Self.TreeKEM.fst
@@ -1,0 +1,325 @@
+module MLS.Test.Self.TreeKEM
+
+open FStar.All
+open Lib.ByteSequence
+open MLS.Crypto
+open MLS.Parser
+open MLS.NetworkTypes
+open MLS.NetworkBinder
+open MLS.Tree
+open MLS.TreeSync.Types
+open MLS.TreeSync.Extensions
+open MLS.TreeSync.ExternalPath
+open MLS.TreeSync
+open MLS.TreeSync.Hash
+open MLS.TreeKEM
+open MLS.TreeMath
+open MLS.TreeSyncTreeKEMBinder
+open MLS.Test.Utils
+open MLS.Result
+
+type participant_secrets (cs:ciphersuite) = {
+  sign_sk: sign_private_key cs;
+  leaf_secret: lbytes (hpke_private_key_length cs);
+}
+
+type mls_state (cs:ciphersuite) = {
+  public: state_t;
+  secrets: list (nat & participant_secrets cs);
+}
+
+type test_state = {
+  n_add: nat;
+  n_update: nat;
+  n_remove: nat;
+}
+
+type state (cs:ciphersuite) = {
+  rng: rand_state;
+  mls: mls_state cs;
+  test: test_state;
+}
+
+type op_type = | Add | Update | Remove
+
+val dumb_credential: credential_t
+let dumb_credential = {
+  version = 0;
+  identity = Seq.empty;
+  signature_key = Seq.empty;
+}
+
+val get_secret: #a:Type -> list (nat & a) -> nat -> ML a
+let rec get_secret #a l x =
+  extract_result (from_option "" (List.Tot.assoc x l))
+
+val update_secret: #a:Type -> list (nat & a) -> (nat & a) -> ML (list (nat & a))
+let rec update_secret #a l (x, s) =
+  match l with
+  | [] -> failwith "remove_secret: couldn't find index"
+  | (hx, hs)::t ->
+    if hx = x then
+      (x,s)::t
+    else
+      (hx,hs)::(update_secret t (x,s))
+
+val remove_secret: #a:Type -> list (nat & a) -> nat -> ML (list (nat & a))
+let rec remove_secret #a l x =
+  match l with
+  | [] -> failwith "remove_secret: couldn't find index"
+  | (hx, hs)::t ->
+    if hx = x then
+      t
+    else
+      (hx,hs)::(remove_secret t x)
+
+//TODO: copy-pasted from MLS.fst
+val gen_leaf_package: #cs:ciphersuite -> rand_state -> participant_secrets cs -> sign_public_key cs -> hpke_public_key cs -> ML (rand_state & leaf_package_t)
+let gen_leaf_package #cs rng secrets sign_pk hpke_pk =
+  let (rng, identity) = gen_rand_bytes rng 8 in
+  let extensions = (
+    let versions = Seq.seq_of_list [PV_mls10] in
+    let ciphersuite_network = extract_result (ciphersuite_to_nt cs) in
+    let ciphersuites = Seq.seq_of_list [ciphersuite_network] in
+    let extensions = Seq.seq_of_list [ET_capabilities; ET_lifetime; (* ET_key_id; *) ET_parent_hash] in
+    if not (byte_length ps_protocol_version (Seq.seq_to_list versions) < 256) then failwith ""
+    else if not (byte_length ps_extension_type (Seq.seq_to_list extensions) < 256) then failwith ""
+    else if not (byte_length ps_cipher_suite (Seq.seq_to_list ciphersuites) < 256) then failwith ""
+    else (
+      let ext = empty_extensions in
+      let ext = extract_result (set_capabilities_extension ext ({versions; ciphersuites; extensions})) in
+      let ext = extract_result (set_lifetime_extension ext ({not_before = Lib.IntTypes.u64 0; not_after = Lib.IntTypes.u64 0})) in
+      ext
+    )
+  ) in
+  let unsigned_leaf_package: leaf_package_t = {
+    credential = {
+      version = 0;
+      identity;
+      signature_key = sign_pk;
+    };
+    version = 0;
+    content = ps_leaf_package_content.serialize ({public_key = hpke_pk});
+    extensions;
+    signature = Seq.empty;
+  } in
+  let (rng, sign_nonce) = gen_rand_bytes rng (sign_nonce_length cs) in
+  let signature = extract_result (
+    unsigned_key_package <-- treesync_to_keypackage cs unsigned_leaf_package;
+    let tbs = ps_key_package_tbs.serialize (key_package_get_tbs unsigned_key_package) in
+    sign_sign cs secrets.sign_sk tbs (mk_randomness sign_nonce)
+  ) in
+  (rng, { unsigned_leaf_package with signature })
+
+val create_participant: cs:ciphersuite -> rand_state -> ML (rand_state & leaf_package_t & participant_secrets cs)
+let create_participant cs rng =
+  let (rng, sign_seed) = gen_rand_bytes rng (sign_private_key_length cs) in
+  let (rng, leaf_secret) = gen_rand_bytes rng (hpke_private_key_length cs) in
+  let (sign_pk, sign_sk) = extract_result (sign_gen_keypair cs (mk_randomness sign_seed)) in
+  let (hpke_sk, hpke_pk) = extract_result (derive_keypair_from_path_secret cs leaf_secret) in
+  let my_secrets = {sign_sk; leaf_secret} in
+  let (rng, leaf_package) = gen_leaf_package rng my_secrets sign_pk hpke_pk in
+  (rng, leaf_package, my_secrets)
+
+val add_rand: #cs:ciphersuite -> rand_state -> mls_state cs -> ML (rand_state & mls_state cs)
+let add_rand #cs rng st =
+  let (rng, leaf_package, my_secrets) = create_participant cs rng in
+  let (new_public_state, leaf_index) = MLS.TreeSync.add st.public dumb_credential leaf_package in
+  (rng, {
+    public = new_public_state;
+    secrets = (leaf_index, my_secrets) :: st.secrets;
+  })
+
+//TODO: the group context is replaced with only the tree hash
+#push-options "--z3rlimit 50"
+val update_leaf: #cs:ciphersuite -> rand_state -> mls_state cs -> nat -> ML (rand_state & mls_state cs)
+let update_leaf #cs rng st leaf_index =
+  let leaf_secrets = get_secret st.secrets leaf_index in
+  if not (leaf_index < st.public.treesize) then failwith "" else
+  let tree_ts = st.public.tree in
+  let tree_tk = extract_result (treesync_to_treekem cs tree_ts) in
+  let (rng, new_leaf_secret) = gen_rand_bytes rng (hpke_private_key_length cs) in
+  let ad = extract_result (tree_hash cs (root st.public.levels) tree_ts) in
+  let rand_length = (update_path_entropy_length tree_tk leaf_index) in
+  if not (rand_length < Lib.IntTypes.max_size_t) then failwith "" else
+  let (rng, rand_bytes) = gen_rand_bytes rng rand_length in
+  let rand = mk_randomness rand_bytes in
+  let (path_tk, _) = extract_result (update_path tree_tk leaf_index new_leaf_secret ad rand) in
+  let leaf_package =
+    match get_leaf tree_ts leaf_index with
+    | (_, Some lp) -> lp
+    | _ -> failwith ""
+  in
+  let ext_path_ts = extract_result (treekem_to_treesync leaf_package path_tk) in
+  let (rng, sign_nonce_bytes) = gen_rand_bytes rng (sign_nonce_length cs) in
+  let sign_nonce = mk_randomness #(sign_nonce_length cs) sign_nonce_bytes in
+  let path_ts = extract_result (external_pathsync_to_pathsync cs (Some (leaf_secrets.sign_sk, sign_nonce)) tree_ts ext_path_ts) in
+  let new_tree_ts = apply_path dumb_credential tree_ts path_ts in
+  (rng, {
+    public = {
+      st.public with
+      tree = new_tree_ts;
+      version = st.public.version + 1;
+    };
+    secrets = update_secret st.secrets (leaf_index, {leaf_secrets with leaf_secret = new_leaf_secret});
+  })
+#pop-options
+
+val update_rand: #cs:ciphersuite -> rand_state -> mls_state cs -> ML (rand_state & mls_state cs)
+let update_rand #cs rng st =
+  let (rng, i) = gen_rand_num_ml rng (List.Tot.length st.secrets) in
+  let (leaf_index, _) = List.Tot.index st.secrets i in
+  update_leaf rng st leaf_index
+
+val remove_leaf: #cs:ciphersuite -> rand_state -> mls_state cs -> nat -> ML (rand_state & mls_state cs)
+let remove_leaf #cs rng st leaf_index =
+  if not (leaf_index < st.public.treesize) then failwith "" else
+  (rng, {
+    public = remove st.public dumb_credential leaf_index;
+    secrets = List.Tot.filter (fun (x, _) -> x <> leaf_index) st.secrets;
+  })
+
+val remove_rand: #cs:ciphersuite -> rand_state -> mls_state cs -> ML (rand_state & mls_state cs)
+let remove_rand #cs rng st =
+  let (rng, i) = gen_rand_num_ml rng (List.Tot.length st.secrets) in
+  let (leaf_index, _) = List.Tot.index st.secrets i in
+  remove_leaf rng st leaf_index
+
+val apply_random_operation: #cs:ciphersuite -> state cs -> ML (state cs & bool)
+let apply_random_operation #cs st =
+  let rng = st.rng in
+  let (rng, op) =
+    if 2 <= List.Tot.length st.mls.secrets then (
+      let (rng, choice) = gen_rand_num_ml rng (st.test.n_add + st.test.n_update + st.test.n_remove) in
+      (rng, (
+        if choice < st.test.n_add then Add
+        else if choice < st.test.n_add + st.test.n_update then Update
+        else Remove
+      ))
+    ) else (
+      let (rng, choice) = gen_rand_num_ml rng (st.test.n_add + st.test.n_update) in
+      (rng, (
+        if choice < st.test.n_add then Add
+        else Update
+      ))
+    )
+  in
+  //assert (op == Add ==> 0 < st.test.n_add);
+  //assert (op == Update ==> 0 < st.test.n_update);
+  //assert (op == Remove ==> 0 < st.test.n_remove);
+  match op with
+  | Add -> (
+    let (rng, mls) = add_rand rng st.mls in
+    ({rng; mls; test={st.test with n_add = st.test.n_add - 1}}, false)
+  )
+  | Update -> (
+    let (rng, mls) = update_rand rng st.mls in
+    ({rng; mls; test={st.test with n_update = st.test.n_update - 1}}, true)
+  )
+  | Remove -> (
+    let (rng, mls) = remove_rand rng st.mls in
+    ({rng; mls; test={st.test with n_remove = st.test.n_remove - 1}}, false)
+  )
+
+val check_root_secret: #cs:ciphersuite -> mls_state cs -> ML unit
+let check_root_secret #cs st =
+  let open MLS.TreeKEM.Types in
+  let (first_index, first_secret) = List.hd st.secrets in
+  let tree_tk = extract_result (treesync_to_treekem cs st.public.tree) in
+  //IO.print_string (
+  //  print_tree
+  //    (fun leaf -> match leaf with
+  //      | None -> "_"
+  //      | Some _ -> "L")
+  //    (fun node -> match node with
+  //      | None -> "_"
+  //      | Some np -> "N[" ^ list_to_string nat_to_string np.unmerged_leafs ^ ", " ^ (if np.path_secret_from = Left then "Left" else "Right") ^ ", " ^ nat_to_string (List.Tot.length np.path_secret_ciphertext) ^ "]")
+  //    tree_tk
+  //);
+  //IO.print_string "\n";
+  if not (first_index < st.public.treesize) then failwith "" else
+  let first_root_secret = extract_result (root_secret tree_tk first_index first_secret.leaf_secret) in
+  List.iter #(nat & participant_secrets cs) (fun (index, secret) ->
+    if not (index < st.public.treesize) then failwith "" else
+    let cur_root_secret = extract_result (root_secret tree_tk index secret.leaf_secret) in
+    if not (first_root_secret = cur_root_secret) then
+      failwith ("check_root_secret: " ^ nat_to_string first_index ^ " has " ^ bytes_to_hex_string first_root_secret ^ ", " ^ nat_to_string index ^ " has " ^ bytes_to_hex_string cur_root_secret)
+    else
+      ()
+  ) (List.tail st.secrets)
+
+val foldn: #a:Type -> nat -> (a -> ML a) -> a -> ML a
+let rec foldn nb f x =
+  if nb = 0 then (
+    x)
+  else (
+    foldn (nb-1) f (f x)
+  )
+
+val create_init_state: cs:ciphersuite -> nat -> ML (rand_state & mls_state cs)
+let create_init_state cs seed =
+  let rng = init_rand_state seed in
+  let (rng, _) = gen_rand_bytes rng 64 in // Avoid the first bad number generation (might not be useful, but doesn't hurt)
+  let (rng, group_id) = gen_rand_bytes rng 16 in
+  let (rng, first_leaf_package, first_secrets) = create_participant cs rng in
+  (rng, ({
+    public = create group_id first_leaf_package;
+    secrets = [(0, first_secrets)];
+  }))
+
+val run_one_self_treekem_test: ciphersuite -> nat -> nat -> nat -> nat -> ML unit
+let run_one_self_treekem_test cs seed avg_n_participant n_remove n_update =
+  IO.print_string ("Running treekem tests with parameters " ^
+    "seed=" ^ (nat_to_string seed) ^ ", " ^
+    "avg_n_participant=" ^ (nat_to_string avg_n_participant) ^ ", " ^
+    "n_remove=" ^ (nat_to_string n_remove) ^ ", " ^
+    "n_update=" ^ (nat_to_string n_update) ^ "\n"
+  );
+  let (rng, mls) = create_init_state cs seed in
+  let init_state = {
+    rng;
+    mls;
+    test = {
+      n_add = avg_n_participant + n_remove;
+      n_update;
+      n_remove;
+    };
+  } in
+  let (_: state cs) = foldn (avg_n_participant + n_remove + n_update + n_remove) (fun st ->
+    let (st, check) = apply_random_operation st in
+    (if check then check_root_secret #cs st.mls else ());
+    st
+  ) init_state in
+  ()
+
+val custom_test_1: ciphersuite -> ML unit
+let custom_test_1 cs =
+  let (rng, st) = create_init_state cs 0 in
+  let (rng, st) = add_rand rng st in
+  let (rng, st) = add_rand rng st in
+  let (rng, st) = add_rand rng st in
+  let (rng, st) = add_rand rng st in
+  let (rng, st) = update_leaf rng st 1 in
+  let (rng, st) = update_leaf rng st 2 in
+  let (rng, st) = update_leaf rng st 3 in
+  let (rng, st) = update_leaf rng st 4 in
+  let (rng, st) = remove_leaf rng st 2 in
+  let (rng, st) = update_leaf rng st 1 in
+  let (rng, st) = add_rand rng st in
+  let (rng, st) = update_leaf rng st 4 in
+  check_root_secret st
+
+val run_self_treekem_test: unit -> ML unit
+let run_self_treekem_test () =
+  let cs = Success?.v (ciphersuite_from_nt CS_mls10_128_dhkemx25519_chacha20poly1305_sha256_ed25519) in
+  custom_test_1 cs;
+  //                           seed add remove update
+  run_one_self_treekem_test cs 0    5   5      5   ;
+  run_one_self_treekem_test cs 1    5   20     20  ;
+  run_one_self_treekem_test cs 2    5   50     25  ;
+  run_one_self_treekem_test cs 3    10  10     10  ;
+  run_one_self_treekem_test cs 4    10  25     25   ;
+  run_one_self_treekem_test cs 5    10  50     25  ;
+  run_one_self_treekem_test cs 6    25  25     25  ;
+  run_one_self_treekem_test cs 7    50  20     100 ;
+  ()
